\documentclass[letterpage]{article}

\input{../common_preambles}

\begin{document}
\begin{align}
  g(x)&=e^{-a(x-b)^2}\\
  \frac{dg(x)}{dx}& = -2a(x-b)g(x)
\end{align}
Fourier transform pair is defined to be,
\begin{equation}
  G(w) = F\{g(x)\} = \int_{-\infty}^\infty g(x)e^{iwx}dx
\end{equation}
Then,
\begin{equation}
  \frac{dG(w)}{dw} = \int_{-\infty}^\infty ixg(x)e^{iwx}dx = F\{ixg(x)\}
\end{equation}
Taking the Fourier transform of both sides of (1), we get
\begin{align}
  -iwG(w) &= -2a \left(\frac{1}{i} \frac{dG(w)}{dw} - bG(w)\right)\\
  \left(ib-\frac{w}{2a}\right) G(w) &= \frac{dG(w)}{dw} \Rightarrow
  \frac{1}{G(w)} \frac{dG(w)}{dw} = ib-\frac{w}{2a}\\
  \int_0^w \frac{1}{G(w)'} \frac{dG(w)'}{dw'} dw' &= 
  \arrowvert\ln G(w')\arrowvert_0^w = \ln G(w) - \ln G(0) 
  = \ln \frac{G(w)}{G(0)}\\
  \int_0^w \left(ib-\frac{w}{za}\right)dw' &= \arrowvert ibw' - \frac{{w'}^2}{-4a}
  \arrowvert_0^w = ibw-\frac{w^2}{4a}\\
  G(0) = \int_{-\infty}^\infty g(x) dx &= \int_{-\infty}^\infty e^{-a(x-b)^2}
  = \sqrt{\frac{\pi}{a}}
\end{align}
From (2), (3), and (4), we get
\begin{align}
  G(w) = G(0) e^{ibw-\frac{w^2}{4a}} &= \sqrt{\frac{\pi}{a}} \quad e^{ibw} 
  e^{-\frac{w^2}{4a}}\\
  \text{or} \qquad
  \int_{-\infty}^\infty e^{-a(x-b)^2} e^{iqx}dx &= \sqrt{\frac{\pi}{a}}
  \: e^{ibq} e^{-\frac{q^2}{4a}}
\end{align}
\begin{align}
  g(x) &= F^{-1} \{G(w)\} = \frac{1}{2\pi} \int_{-\infty}^\infty 
  G(w)e^{-iwx}dw\\
  \text{and} \qquad \frac{dg(x)}{dx} &= \frac{1}{2\pi} \int_{-\infty}^\infty
  (-iw)G(w)e^{-iwx}dw\\
  &=F^{-1} \left\{-iwG(w)\right\}\\
  &\Rightarrow F\left\{\frac{dg(x)}{dx} \right\} = -(iwG(w))
\end{align}
\\
\begin{equation*}
  u(x) = \left\{
    \begin{array}{ccc}
    -\frac{A}{\lambda_r-X_0}\left(x+\frac{\lambda_r}{2}\right) 
      & \text{for} 
      & -\frac{\lambda_r}{2} \leq x < -\frac{x_0}{2} \\
    \frac{A}{x_0}x 
      & \text{for} 
      & -\frac{x_0}{2} \leq x \leq \frac{x_0}{2} \\
    -\frac{A}{\lambda_r-X_0} \left(x-\frac{\lambda_r}{2}\right)
      & \text{for} 
      & \frac{x_0}{2} < x \leq \frac{\lambda_r}{2}
    \end{array} \right.
\end{equation*}
\begin{align}
  Fc(\textbf{q}) &= \int_{-\frac{\lambda_r}{2}}^{\frac{\lambda_r}{2}}dx
  \int_{-\frac{D}{2}}^\frac{D}{2} dz \: \delta\left(z-u(x)\right)
  e^{iq_zZ} e^{iq_xX} \\
  &= \int_{\frac{-\lambda_r}{2}}^{\frac{\lambda_r}{2}} dx \: e^{iq_zu(x)}
  e^{iq_xX}
\end{align}
\begin{align}
  \int_{-\frac{\lambda_r}{2}}^{-\frac{x_0}{2}} dx \: e^{iq_xx} e^{iq_zu(x)}
  &= -\int_{\frac{\lambda_r}{2}}^{\frac{x_0}{2}} 
  dy \: e^{-iq_xy}e^{iq_zu(-y)}\\
  &= \int_{\frac{x_0}{2}}^{\frac{\lambda_r}{2}} dx \: e^{-iq_xx} 
  e^{iq_z\frac{A}{\lambda_r-x_0}\left(x-\frac{\lambda_r}{2}\right)}\\
  &= \int_{\frac{x_0}{2}}^{\frac{\lambda_r}{2}}dx \: 
  e^{-i\left[q_xx - q_z \frac{A}{\lambda_r-x_0}
  \left(x-\frac{\lambda_r}{2}\right)\right]}
\end{align}
\begin{align}
  \int_{\frac{x_0}{2}}^{\frac{\lambda_r}{2}} dx \: e^{iq_xx} e^{iq_zu(x)}
  = \int_{\frac{x_0}{2}}^{\frac{\lambda_r}{2}} dx \: 
  e^{i\left[q_xx-q_z\frac{A}{\lambda_r-x_0}
  \left(x-\frac{\lambda_r}{2}\right)\right]}
\end{align}
So,
\begin{equation}
  \int_{-\frac{\lambda_r}{2}}^{-\frac{x_0}{2}} dx \:
  e^{i{\left[q_xx+q_zu(x)\right]}}
  + \int_{\frac{x_0}{2}}^{\frac{\lambda_r}{2}} dx \: 
  e^{i\left[q_xx+q_zu(x)\right]}
\end{equation}

\begin{align}
  &= 2\int_{\frac{x_0}{2}}^{\frac{\lambda_r}{2}}   
     \cos\bracks{\pars{q_x-q_z\frac{A}{\lambda_r-x_0}}x
     + q_z\frac{A}{\lambda_r-x_0}\frac{\lambda_r}{2}} \\
  &= \frac{2}{q_x-q_z\frac{A}{\lambda_r-x_0}} 
     \braces{}
\end{align}
Using $\sin u-\sin v = 2\cos[(u+v)/2]\sin[(u-v)/2]$
\begin{align}
  =& \frac{4(\lambda_r-x_0)}{q_x(\lambda_r-x_0)-q_zA}
  \: cos\left[\frac{1}{2} \left(\frac{1}{2}q_x (\lambda_r + x_0)
  + \frac{1}{2} q_zA \right)\right]\\
  & \cdot sin \frac{1}{2} \left(\frac{1}{2}q_x(\lambda_r-x_0)
  -\frac{1}{2}q_zA\right)
\end{align}
Defining $w = \frac{1}{2} \left(q_xx_0 + q_z A \right)$, we get
\begin{align}
  &= \frac{2(\lambda_r-x_0)}{\frac{1}{2}q_x \lambda_r - \frac{1}{2}q_x x_0
  -\frac{1}{2} q_z A} \: cos \frac{1}{2} \left(w + \frac{1}{2}q_x 
  \lambda_r \right) \: sin \frac{1}{2} \left(\frac{1}{2} q_x \lambda_r-w \right)\\
  &= \frac{(\lambda_r-x_0)}{\frac{1}{2}q_x \lambda_r - w} \: cos \frac{1}{2}
  \left(w + \frac{1}{2}q_x \lambda_r \right) 
  \frac{sin\left(\frac{1}{2}q_x \lambda_r - w \right)}
  {cos\frac{1}{2}\left(\frac{1}{2}q_x \lambda_r -w \right)}\\
  &= (\lambda_r - x_0) \frac{cos\frac{1}{2}\left(\frac{1}{2}q_x \lambda_r
  + w \right)}{cos\frac{1}{2} \left(\frac{1}{2} q_x \lambda_r - w \right)}
  \: \frac{sin \left(\frac{1}{2}q_x \lambda_r - w \right)}{\frac{1}{2}
  q_x \lambda_r - w}
\end{align}
\begin{equation}
  \int_{-\frac{x_0}{2}}^{\frac{x_0}{2}} dx \: e^{iq_z \frac{A}{x_0}x}
  e^{iqx} = \int_{-\frac{x_0}{2}}^{\frac{x_0}{2}} dx \: 
  e^{i\left(\frac{q_zA}{x_0} + q_x \right)x}
\end{equation}
\begin{align}
  &= 2 \int_{0}^{\frac{x_0}{2}} dx \:cos \left(\frac{q_zA}{x_0} + q_x \right)x\\
  &= \frac{2}{\frac{q_zA}{x_0} + q_x}
    \sin\left.\left(\frac{q_zA}{x_0} + q_x \right) x \right|_{0}^{\frac{x_0}{2}}\\
  &= \frac{2}{\frac{q_zA}{x_0}+q_x} \: sin \left(\frac{q_zA}{x_0}+q_x \right)
  \frac{x_0}{2}\\
  &= \frac{2x_0}{q_zA + x_0 q_x} \: sin \frac{1}{2} (q_zA + q_z x_0)\\
  &= x_0 \: \frac{sin\frac{1}{2}\left(q_zA + q_x x_0 \right)}
  {\frac{1}{2}\left(q_zA + q_x x_0 \right)}\\
  &= x_0 \frac{sinw}{w}\\
  \therefore & \: F_c(\textbf{q}) = x_0 \frac{sin \:w}{w} + (\lambda_r - x_0)
  \frac{cos\frac{1}{2}\left(\frac{1}{2} q_x \lambda_r + w\right)}
  {cos\frac{1}{2} \left(\frac{1}{2}q_x \lambda_r - w \right)}
  \frac{sin\left(\frac{1}{2}q_x \lambda_r - w \right)}{\frac{1}{2}q_x \lambda_r
  - w}
\end{align}

\begin{equation}
  \pars{\frac{c}{d}}
  \braces{\frac{x}{y}}
  \bracks{\frac{a}{b}}
\end{equation}
\end{document}